src/Core/Solver/TD_Side/TD_Side_CFG.thy
@@ -22,13 +22,32 @@ text \<open>
 
 (* Keep only the local (resp. global) component of an abstract state; the other
    component is set to bot, so the join of the two recovers the original. *)
+definition restrict_local_for ::
+  "(vname => bool) => 'a::bounded_semilattice_sup_bot abs_state => 'a abs_state" where
+  "restrict_local_for gs \<sigma> = (%x. if gs x then bot else \<sigma> x)"
+
+definition restrict_global_for ::
+  "(vname => bool) => 'a::bounded_semilattice_sup_bot abs_state => 'a abs_state" where
+  "restrict_global_for gs \<sigma> = (%x. if gs x then \<sigma> x else bot)"
+
 definition restrict_local ::
   "'a::bounded_semilattice_sup_bot abs_state => 'a abs_state" where
-  "restrict_local \<sigma> = (\<lambda>x. if is_global x then bot else \<sigma> x)"
+  "restrict_local \<sigma> = (%x. if is_global x then bot else \<sigma> x)"
 
 definition restrict_global ::
   "'a::bounded_semilattice_sup_bot abs_state => 'a abs_state" where
-  "restrict_global \<sigma> = (\<lambda>x. if is_global x then \<sigma> x else bot)"
+  "restrict_global \<sigma> = (%x. if is_global x then \<sigma> x else bot)"
+
+lemma restrict_local_for_global_join:
+  "restrict_local_for gs \<sigma> \<squnion> restrict_global_for gs \<sigma> = \<sigma>"
+  unfolding restrict_local_for_def restrict_global_for_def sup_fun_def
+  by (rule ext) simp
+
+lemma restrict_global_for_local_join:
+  "restrict_global_for gs \<sigma> \<squnion> restrict_local_for gs \<sigma> = \<sigma>"
+  unfolding restrict_local_for_def restrict_global_for_def sup_fun_def
+  by (rule ext) simp
+
 
 lemma restrict_local_global_join:
   "restrict_local \<sigma> \<squnion> restrict_global \<sigma> = \<sigma>"
